Rearranging code, made a main.fst.
The code now compiles and is consistent with the communcation diagram specified in the report

Code/AuthenticationProvider.fst
@@ -3,6 +3,8 @@ module Authenticationprovider
 open SamlProtocol
 open Crypto
 open Database
+open TypeFunc
+
 (*
 val createAssertion: me:prin -> user:prin -> Assertion
 
@@ -16,18 +18,25 @@ let createAssertion me user idp =
 	EncryptAssertion idp pubkidp signAssertion
 *)
 
-val nfactauth: me:prin -> idp:prin -> name:string -> assertion:Assertion -> unit
+val relatechallenge: user:prin -> challenge:nonce -> unit
 
-let nfactauth me idp name assertion =
-	if (allnfactauthed name) then
-		resetnfact name;
+val verifychallenge: user:prin -> challenge:nonce -> bool
+
+val nfactauth: me:prin -> idp:prin -> user:prin -> userid:string -> unit
+
+let nfactauth me idp user userid =
+	if (allnfactauthed userid) then
+		resetnfact userid;
 		let status = "OK" in
-		let resp = LoginSuccess status me idp assertion in
+		let resp = LoginSuccess status me idp in
 		SendSaml idp resp
 	else
 		let challenge = GenerateNonce me in
-		let authmethod = getnfactor name in
-		let resp = LoginResponseMessage me idp assertion authmethod challenge in
+		let authmethod = getnfactor userid in
+		assume(LogAuth user authmethod);
+		let userprivkey = CertStore.GetPrivateKey user in
+		let sigUser = SignAuth user userprivkey authmethod in
+		let resp = LoginResponseMessage me idp authmethod challenge sigUser in
 		SendSaml idp resp
 
 val authenticationprovider: me:prin -> idp:prin -> user:prin -> unit
@@ -35,24 +44,18 @@ val authenticationprovider: me:prin -> idp:prin -> user:prin -> unit
 let rec authenticationprovider me idp user =
 	let req = ReceiveSaml idp in
 	match req with
-	| LoginRequestMessage (issuer, destination, message, loginInfo, sigIdP) ->
-		let pubkissuer = CertStore.GetPublicKey issuer in
-		if (whitelisted idp) && (VerifySignature issuer pubkissuer message sigIdP) then
-			(assert (Log issuer message);
+	| LoginRequestMessage (issuer, destination, loginInfo) ->
+		if (whitelisted idp) then
 			match loginInfo with
-			| UserLogin(name, password) ->
-				if not (revokedidp name idp) && (checklogin name password) then
-					(*Find the n-factor auth method - How / which one if more?*)
+			| UserLogin(userid, password) ->
+				if not (revokedidp userid idp) && (checklogin userid password) then
 					let challenge = GenerateNonce me in
-					let assertion = MakeAssertion me user idp in
-					let myprivk = CertStore.GetPrivateKey me in
-					assume(Log me assertion);
-					let pubkidp = CertStore.GetPublicKey idp in
-					let sigAs = Sign me myprivk assertion in
-					let signAssertion = AddSignatureToAssertion assertion sigAs in
-					let assertion = EncryptAssertion idp pubkidp signAssertion in
-					let authmethod = getnfactor name in
-					let resp = LoginResponseMessage me idp assertion authmethod challenge in
+					let authmethod = getnfactor userid in
+					assume(LogAuth user authmethod);
+					let userprivkey = CertStore.GetPrivateKey user in
+					let sigUser = SignAuth user userprivkey authmethod in
+					relatechallenge user challenge;
+					let resp = LoginResponseMessage me idp authmethod challenge sigUser in
 					SendSaml idp resp;
 					authenticationprovider me idp user
 				else
@@ -60,34 +63,38 @@ let rec authenticationprovider me idp user =
 					authenticationprovider me idp user
 			| _ -> SendSaml idp (Failed Requester);
 				authenticationprovider me idp user
-			)
 		else
 			SendSaml idp (Failed Requester);
 			authenticationprovider me idp user
-	| NfactAuthRequest(issuer, destination, message, authInfo, challenge, sigIdP)->
-		(*Associate the challenge to the challenge generated at the first login*)
-		let pubkissuer = CertStore.GetPublicKey issuer in
-		if (whitelisted idp) && (VerifySignature issuer pubkissuer message sigIdP) then
-			(assert (Log issuer message);
+	| NfactAuthRequest(issuer, destination, authInfo, challenge, sigAuth) ->
+		if (whitelisted idp) then
 			match authInfo with
-			| UserAuth(name, auth) ->
-				if not (revokedidp name idp) && (checknfactor name auth) then
-					let assertion = MakeAssertion me user idp in
-					let myprivk = CertStore.GetPrivateKey me in
-					assume(Log me assertion);
-					let pubkidp = CertStore.GetPublicKey idp in
-					let sigAs = Sign me myprivk assertion in
-					let signAssertion = AddSignatureToAssertion assertion sigAs in
-					let assertion = EncryptAssertion idp pubkidp signAssertion in
-					nfactauth me name idp assertion;
-					authenticationprovider me idp user
+			| UserAuth(userid, authmethod, authresponse) ->
+				let userpubkey = CertStore.GetPublicKey user in
+				if VerifySignatureAuth user userpubkey authmethod sigAuth && verifychallenge user challenge then
+					if not (revokedidp userid idp) && (checknfactor userid authresponse) then
+						nfactauth me idp user userid;
+						authenticationprovider me idp user
+					else
+						SendSaml idp (Failed User);
+						authenticationprovider me idp user
 				else
 					SendSaml idp (Failed User);
 					authenticationprovider me idp user
 			| _ -> SendSaml idp (Failed Requester);
-				authenticationprovider me idp user)
+				authenticationprovider me idp user
 		else
 			SendSaml idp (Failed Requester);
 			authenticationprovider me idp user
 	| _ -> SendSaml idp (Failed Requester);
 		authenticationprovider me idp user
+
+val usercommunication: me:prin -> user:prin -> unit
+
+(*
+let rec authenticationprovider me user =
+	let req = ReceiveSaml idp in
+	match req with
+	| UserRequest -> do something
+	| _ -> SendSaml user (DisplayError 400);
+		usercommunication me user*)
