Code/Crypto.fst
@@ -1,6 +1,8 @@
 module Crypto
 
 open Protocol
+open TypeFunc
+
 type prin = string
 type pubkey :: prin => *
 type privkey :: prin => *
@@ -11,6 +13,8 @@ type cypher
 (*Verification*)
 type Log :: prin => string => E
 
+type LogAuth :: prin => Authentication => E
+
 val Keygen: p:prin
           -> (pubkey p * privkey p)
 
@@ -19,11 +23,22 @@ val Sign: p:prin
         -> msg:string{Log p msg}
         -> dsig
 
+val SignAuth: p:prin
+        -> privkey p
+        -> msg:Authentication{LogAuth p msg}
+        -> dsig
+
 val VerifySignature: p:prin
         -> pubkey p 
         -> msg:string
         -> dsig
         -> b:bool{b=true ==> Log p msg}
+
+val VerifySignatureAuth: p:prin
+        -> pubkey p 
+        -> msg:Authentication
+        -> dsig
+        -> b:bool{b=true ==> LogAuth p msg}
 
 val Encrypt: p:prin
         -> pubkey p
