Code/IdentityProvider.fst
@@ -2,6 +2,7 @@ module Identityprovider
 
 open SamlProtocol
 open Crypto
+open TypeFunc
 
 (*type SecurityRestriction = 
 	| Session: 1
@@ -13,22 +14,24 @@ type SecurityProfile =
 				int -> SecurityProfile
 *)
 
+val userloggedin: user:prin -> bool
+val getjavascript: string
+val decodeMessage: message:string -> AuthnRequest
 val getauthnrequest: user:prin -> challenge:nonce -> AuthnRequest
 val getuserchallenge: user:prin -> nonce
 val relatechallenge: user:prin -> challenge:nonce -> unit
+val verifychallenge: user:prin -> challenge:nonce -> bool
 val relate: user:prin -> challenge:nonce -> authnReq:AuthnRequest -> unit
-val generateid: id
-val timestamp: string
 
 val handleUserAuthenticated: me:prin -> user:prin -> authnReq:AuthnRequest -> unit
 
 let handleUserAuthenticated me user authnReq = 
 	match authnReq with
-	| MkAuthnRequest(reqid,issueinst,dest,sp,msg,sigSP) ->
+	| MkAuthnRequest(issueinst,dest,sp,msg,sigSP) ->
 		let pubksp = CertStore.GetPublicKey sp in
 			if (VerifySignature sp pubksp msg sigSP) then
         	(assert (Log sp msg);
-        	let assertion = IssueAssertion me user sp reqid in
+        	let assertion = IssueAssertion me user sp authnReq in
         	let myprivk = CertStore.GetPrivateKey me in
         	assume(Log me assertion);
         	let sigAs = Sign me myprivk assertion in
@@ -44,32 +47,22 @@ val handleauthresponse: me:prin -> user:prin -> authp:prin -> unit
 let handleauthresponse me user authp =
 	let resp = ReceiveSaml authp in
 	match resp with
-	| LoginResponseMessage(issuer, destination, encassertion, authmethod, challenge) ->
-		let meprivk = CertStore.GetPrivateKey me in
-		let assertion = DecryptAssertion me meprivk encassertion in
-		match assertion with
-		| SignedAssertion(token, sigAuthP) ->
-			let pubkissuer = CertStore.GetPublicKey authp in
-			if VerifySignature authp pubkissuer token sigAuthP then
-				(assert (Log authp token);
-				relatechallenge user challenge;
-				let resp = UserAuthRequest authmethod challenge in
-				SendSaml user resp)
-			else SendSaml user (DisplayError 403)
-		| _ -> SendSaml user (DisplayError 400)
-	| LoginSuccess(status, issuer, destination, encassertion) ->
-		let meprivk = CertStore.GetPrivateKey me in
-		let assertion = DecryptAssertion me meprivk encassertion in
-		match assertion with
-		| SignedAssertion(token, sigAuthP) ->
-			let pubkissuer = CertStore.GetPublicKey authp in
-			if (status = "OK") && (VerifySignature authp pubkissuer token sigAuthP) then
-				(assert (Log authp token);
-				let challenge = getuserchallenge user in
-				let authnReq = getauthnrequest user challenge in
-				handleUserAuthenticated me user authnReq)
-			else SendSaml user (DisplayError 403)
-		| _ -> SendSaml user (DisplayError 400)
+	| LoginResponseMessage(issuer, destination, authmethod, challenge, sigUser) ->
+		let pubkeyuser = CertStore.GetPublicKey user in
+		if VerifySignatureAuth user pubkeyuser authmethod sigUser then
+			(assert (LogAuth user authmethod);
+			relatechallenge user challenge;
+			let resp = UserAuthRequest authmethod challenge sigUser in
+			SendSaml user resp)
+		else
+			SendSaml user (DisplayError 403)
+	| LoginSuccess(status, issuer, destination) ->
+		if (status = "OK") then
+			let challenge = getuserchallenge user in
+			let authnReq = getauthnrequest user challenge in
+			handleUserAuthenticated me user authnReq
+		else 
+			SendSaml user (DisplayError 403)
 	| _ -> SendSaml user (DisplayError 400)
 
 val identityprovider: me:prin -> user:prin -> authp:prin -> unit
@@ -81,33 +74,43 @@ let rec identityprovider me user authp =
 		let pubkissuer = CertStore.GetPublicKey issuer in
     	if (VerifySignature issuer pubkissuer message sigSP) then
       		(assert (Log issuer message);
-      		let id = generateid in
-      		let issueinstant = timestamp in
-      		let authnReq = MkAuthnRequest id issueinstant me issuer message sigSP in
-      		let challenge = GenerateNonce me in
-      		relate user challenge authnReq;
-      		relatechallenge user challenge;
-      		let resp = UserCredRequest challenge in
-      		SendSaml user resp;
-      		identityprovider me user authp)
+      		let authnReq = decodeMessage message in
+      		let myprivk = CertStore.GetPrivateKey me in
+      		if not (userloggedin user) then
+      			let challenge = GenerateNonce me in
+      			relate user challenge authnReq;
+      			relatechallenge user challenge;
+      			let js = getjavascript in
+      			assume(Log me js);
+      			let myprivk = CertStore.GetJSPrivateKey me in
+      			let sigIdP = Sign me myprivk js in
+      			let resp = UserCredRequest js challenge sigIdP in
+      			SendSaml user resp;
+      			identityprovider me user authp
+      		else
+      			let assertion = IssueAssertion me user issuer authnReq in
+        		assume(Log me assertion);
+        		let myprivk = CertStore.GetPrivateKey me in
+        		let pubksp = CertStore.GetPublicKey issuer in
+        		let sigAs = Sign me myprivk assertion in
+        		let signAssertion = AddSignatureToAssertion assertion sigAs in
+        		let encryptedAssertion = EncryptAssertion issuer pubksp signAssertion in
+        		let resp = AuthResponseMessage me issuer encryptedAssertion in
+        		SendSaml user resp)
     	else
       		SendSaml user (Failed Requester);
       		identityprovider me user authp
 	| Login (loginInfo, challenge) ->
-		let loginReq = CreateLoginRequestMessage me authp in
-		assume(Log me loginReq);
-		let myprivk = CertStore.GetPrivateKey me in
-		let sigIdP = Sign me myprivk loginReq in
-		let req = LoginRequestMessage me authp loginReq loginInfo sigIdP in
-		SendSaml authp req;
-		handleauthresponse me user authp;
-		identityprovider me user authp
-	| UserAuthResponse(authInfo, challenge) ->
-		let authReq = CreateSecondAuthReqMessage me authp in
-		assume(Log me authReq);
-		let myprivk = CertStore.GetPrivateKey me in
-		let sigIdP = Sign me myprivk authReq in
-		let req = NfactAuthRequest me authp authReq authInfo challenge sigIdP in
+		if (verifychallenge user challenge) then
+			let req = LoginRequestMessage me authp loginInfo in
+			SendSaml authp req;
+			handleauthresponse me user authp;
+			identityprovider me user authp
+		else
+			SendSaml user (DisplayError 400);
+			identityprovider me user authp
+	| UserAuthResponse(authInfo, challenge, sigAuth) ->
+		let req = NfactAuthRequest me authp authInfo challenge sigAuth in
 		SendSaml authp req;
 		handleauthresponse me user authp;
 		identityprovider me user authp
