Code/certstore.fst
@@ -6,3 +6,4 @@ val GetPublicKey: p:prin -> pubkey p
 
 (*Prin needs to be updated to include credentials*)
 val GetPrivateKey: p:prin -> privkey p 
+val GetJSPrivateKey: p:prin -> privkey p
